updated polyId ex

dev2015/dot20.v
@@ -899,38 +899,48 @@ Ltac crush2 :=
 
 (* define polymorphic identity function *)
 
-Definition polyId := TAll (TBind (TMem 0 TBot TTop)) (TFun 0 (TSel (varB 0) 0) (TSel (varB 0) 0)).
+Definition polyId := TAll 0 (TBind (TMem 0 TBot TTop)) (TAll 0 (TSel (varB 0) 0) (TSel (varB 1) 0)).
 
-Example ex1: has_type [] (ttabs 0 (TBind (TMem 0 TBot TTop)) (tlet 1 (tobj 1 [(0, (dfun 2 (tvar 2)))]) (tvar 1))) polyId.
+Example ex1: has_type [] (tlet 0 (tobj 0 [(0, dfun 1 (tlet 2 (tobj 2 [(0, (dfun 3 (tvar 3)))]) (tvar 2)))]) (tvar 0)) polyId.
 Proof.
-  eapply t_tabs.
-  unfold open. simpl. apply t_let with (Tx:=(TBind (TFun 0 (TSel (varF 0) 0) (TSel (varF 0) 0)))); crush2.
-  assert ((open (varF 1) (TFun 0 (TSel (varF 0) 0) (TSel (varF 0) 0)))=(TFun 0 (TSel (varF 0) 0) (TSel (varF 0) 0))) as A. { unfold open. simpl. reflexivity. }
+  apply t_let with (Tx:=(TBind polyId)).
+  apply t_obj with (TX:=polyId).
+  eauto. compute. reflexivity.
+  eapply dt_fun with (T1:=(TBind (TMem 0 TBot TTop))) (T2:=TAll 0 (TSel (varB 0) 0) (TSel (varB 1) 0)).
+  unfold open. simpl. apply t_let with (Tx:=(TBind (TAll 0 (TSel (varF 0) 0) (TSel (varF 0) 0)))); crush2.
+  assert ((open (varF 2) (TAll 0 (TSel (varF 0) 0) (TSel (varF 0) 0)))=(TAll 0 (TSel (varF 0) 0) (TSel (varF 0) 0))) as A. { unfold open. simpl. reflexivity. }
   rewrite <- A at 2.
   eapply t_var_unpack; crush2.
-  crush2.
-  crush2.
+  eapply dt_nil.
+  crush2. crush2. crush2.
+  unfold polyId. crush2. unfold polyId. crush2. crush2.
+  assert (open (varF 0) polyId=polyId) as A. { unfold open. simpl. reflexivity. }
+  rewrite <- A at 2.
+  eapply t_var_unpack; crush2.
+  unfold polyId. crush2.
 Qed.
 
 
 (* instantiate it to bool *)
 
-Example ex2: has_type [(0,polyId)] (ttapp (tvar 0) (tlet 1 (tobj 1 [(0,dmem TBool)]) (tvar 1))) (TFun 0 TBool TBool).
+Example ex2: has_type [(0,polyId)] (tapp (tvar 0) 0 (tlet 1 (tobj 1 [(0,dmem TBool)]) (tvar 1))) (TAll 0 TBool TBool).
 Proof.
-  eapply t_tapp. instantiate (1:= (TBind (TMem 0 TBool TBool))).
+  eapply t_app. instantiate (1:= (TBind (TMem 0 TBool TBool))).
     { eapply t_sub.
       { eapply t_var. simpl. eauto. crush2. }
-      { eapply stp_all; eauto. { eapply stp_bindx; crush2. } compute. eapply cl_fun; eauto.
-        eapply stp_fun. compute. eapply stp_selax; crush2. crush2.
-        eapply stp_fun. compute. eapply stp_selab2. crush2.
+      { eapply stp_all; eauto. { eapply stp_bindx; crush2. } compute. eapply cl_all; eauto.
+        eapply stp_all. compute. eapply stp_selax; crush2. crush2. crush2. crush2.
+        simpl. unfold open. simpl. eapply stp_selax; crush2. crush2.
+        eapply stp_all. compute. eapply stp_selab2. crush2.
         crush2. instantiate (1:=TBool). crush2.
         instantiate (1:=[(0, TBind (TMem 0 TBool TBool))]). simpl. reflexivity.
         rewrite app_nil_l. reflexivity.
-        crush2. crush2. crush2.
+        crush2. crush2. crush2. crush2. crush2. crush2. crush2.
+        simpl. unfold open.
         simpl. eapply stp_selab1. crush2.
         crush2. instantiate (1:=TBool). crush2.
         instantiate (1:=[(0, TBind (TMem 0 TBool TBool))]). simpl. reflexivity.
-        rewrite app_nil_l. reflexivity.
+        instantiate (1:=[(0, TBool)]). simpl. reflexivity.
         crush2. crush2. crush2.
       }
     }
